small changes to replace specs

code/ecdsap256sha2/Hacl.Impl.P256.Arithmetics.fst
@@ -19,6 +19,7 @@ open Hacl.Spec.P256.MontgomeryMultiplication
 
 open FStar.Math.Lemmas
 friend Hacl.Spec.P256.MontgomeryMultiplication
+open Spec.P256.Field
 
 open FStar.Mul
 
@@ -28,8 +29,8 @@ let quatre a result =
     let h0 = ST.get() in 
   montgomery_multiplication_buffer a a result;
   montgomery_multiplication_buffer result result result;
-    inDomain_mod_is_not_mod ((fromDomain_ (as_nat h0 a) * fromDomain_ (as_nat h0 a) % prime256) * (fromDomain_ (as_nat h0 a) * fromDomain_ (as_nat h0 a) % prime256));
-    modulo_distributivity_mult2 (fromDomain_ (as_nat h0 a) * fromDomain_ (as_nat h0 a)) (fromDomain_ (as_nat h0 a) * fromDomain_ (as_nat h0 a)) 1 prime256;
+    inDomain_mod_is_not_mod ((fromDomain_ (as_nat h0 a) * fromDomain_ (as_nat h0 a) % prime) * (fromDomain_ (as_nat h0 a) * fromDomain_ (as_nat h0 a) % prime));
+    modulo_distributivity_mult2 (fromDomain_ (as_nat h0 a) * fromDomain_ (as_nat h0 a)) (fromDomain_ (as_nat h0 a) * fromDomain_ (as_nat h0 a)) 1 prime;
     lemma_brackets (fromDomain_ (as_nat h0 a) * fromDomain_ (as_nat h0 a)) (fromDomain_ (as_nat h0 a)) (fromDomain_ (as_nat h0 a));
     inDomain_mod_is_not_mod (fromDomain_ (as_nat h0 a) * fromDomain_ (as_nat h0 a) * fromDomain_ (as_nat h0 a) * fromDomain_ (as_nat h0 a))
 
@@ -44,10 +45,10 @@ let multByThree a result =
     let h0 = ST.get() in 
   multByTwo a result;
     let h1 = ST.get() in 
-      assert(as_nat h1 result == toDomain_ (2 * fromDomain_ (as_nat h0 a) % prime256));
+      assert(as_nat h1 result == toDomain_ (2 * fromDomain_ (as_nat h0 a) % prime));
   p256_add a result result;
     let h2 = ST.get() in 
-    lemma_mod_add_distr (fromDomain_ (as_nat h0 a)) (2 * fromDomain_ (as_nat h0 a)) prime256;
+    lemma_mod_add_distr (fromDomain_ (as_nat h0 a)) (2 * fromDomain_ (as_nat h0 a)) prime;
     inDomain_mod_is_not_mod (3 * fromDomain_ (as_nat h0 a))
   
 
@@ -55,7 +56,7 @@ let multByFour a result  =
     let h0 = ST.get() in 
   multByTwo a result;
   multByTwo result result;
-    lemma_mod_mul_distr_r 2 (2 * fromDomain_ (as_nat h0 a)) prime256;
+    lemma_mod_mul_distr_r 2 (2 * fromDomain_ (as_nat h0 a)) prime;
     lemma_brackets 2 2 (fromDomain_ (as_nat h0 a)); 
     inDomain_mod_is_not_mod (4 * fromDomain_ (as_nat h0 a))
 
@@ -64,11 +65,11 @@ let multByEight a result  =
     let h0 = ST.get() in 
   multByTwo a result;
   multByTwo result result;
-    lemma_mod_mul_distr_r 2 (2 * fromDomain_ (as_nat h0 a)) prime256;
+    lemma_mod_mul_distr_r 2 (2 * fromDomain_ (as_nat h0 a)) prime;
     lemma_brackets 2 2 (fromDomain_ (as_nat h0 a)); 
     inDomain_mod_is_not_mod (4 * fromDomain_ (as_nat h0 a));
   multByTwo result result;
-    lemma_mod_mul_distr_r 2 (4 * fromDomain_ (as_nat h0 a)) prime256;
+    lemma_mod_mul_distr_r 2 (4 * fromDomain_ (as_nat h0 a)) prime;
     lemma_brackets 2 4 (fromDomain_ (as_nat h0 a));
     inDomain_mod_is_not_mod (8 * fromDomain_ (as_nat h0 a))
 
@@ -80,9 +81,9 @@ let multByMinusThree a result  =
     let zeros = create (size 4) (u64 0) in 
     p256_sub zeros result result;
       lemmaFromDomain 0; 
-      assert_norm( 0 * modp_inv2 (pow2 256) % prime256 == 0);
+      assert_norm( 0 * modp_inv2 (pow2 256) % prime == 0);
       assert_norm (fromDomain_ 0 == 0); 
-      lemma_mod_sub_distr 0 (3 * fromDomain_ (as_nat h0 a)) prime256;
+      lemma_mod_sub_distr 0 (3 * fromDomain_ (as_nat h0 a)) prime;
       inDomain_mod_is_not_mod ((-3) * fromDomain_ (as_nat h0 a));  
   pop_frame()
 
