code/ecdsap256sha2/Hacl.Impl.P256.LowLevel.fst
@@ -18,12 +18,13 @@ open FStar.Math.Lemmas
 open FStar.Mul
 open Lib.IntTypes.Intrinsics
 
+open Spec.P256.Field
+
 #reset-options " --z3rlimit 300"
 
-
 inline_for_extraction
-let prime256_buffer: x: ilbuffer uint64 (size 4) {witnessed #uint64 #(size 4) x (Lib.Sequence.of_list p256_prime_list) /\ recallable x /\ felem_seq_as_nat (Lib.Sequence.of_list (p256_prime_list)) == prime256} = 
-  assert_norm (felem_seq_as_nat (Lib.Sequence.of_list (p256_prime_list)) == prime256);
+let prime256_buffer: x: ilbuffer uint64 (size 4) {witnessed #uint64 #(size 4) x (Lib.Sequence.of_list p256_prime_list) /\ recallable x /\ felem_seq_as_nat (Lib.Sequence.of_list (p256_prime_list)) == prime} = 
+  assert_norm (felem_seq_as_nat (Lib.Sequence.of_list (p256_prime_list)) == prime);
   createL_global p256_prime_list
 
 
@@ -31,10 +32,10 @@ inline_for_extraction noextract
 val reduction_prime256_2prime256_with_carry_impl: cin: uint64 -> x: felem -> result: felem ->
   Stack unit 
     (requires fun h -> live h x /\ live h result /\  eq_or_disjoint x result /\ 
-      (as_nat h x + uint_v cin * pow2 256) < 2 * prime256)
+      (as_nat h x + uint_v cin * pow2 256) < 2 * prime)
     (ensures fun h0 _ h1 -> 
       modifies (loc result) h0 h1 /\ 
-      as_nat h1 result = (as_nat h0 x + uint_v cin * pow2 256) % prime256
+      as_nat h1 result = (as_nat h0 x + uint_v cin * pow2 256) % prime
     )  
 
 
@@ -46,38 +47,36 @@ let reduction_prime256_2prime256_with_carry_impl cin x result =
     let c = sub4_il x prime256_buffer tempBuffer in
   let h0 = ST.get() in 
       assert(uint_v c <= 1);
-      assert(if uint_v c = 0 then as_nat h0 x >= prime256 else as_nat h0 x < prime256);
+      assert(if uint_v c = 0 then as_nat h0 x >= prime else as_nat h0 x < prime);
     let carry = sub_borrow_u64 c cin (u64 0) tempBufferForSubborrow in 
     cmovznz4 carry tempBuffer x result;
   let h1 = ST.get() in 
       assert_norm (pow2 64 * pow2 64 * pow2 64 * pow2 64 = pow2 256);
-      assert_norm (prime256 < pow2 256);
-      assert_norm(pow2 256 < 2 * prime256);
+      assert_norm(pow2 256 < 2 * prime);
 
       assert(uint_v cin <= 1);
       assert(uint_v c <= 1);
 
-      assert(if as_nat h0 x >= prime256 then uint_v c = 0 else True);
+      assert(if as_nat h0 x >= prime then uint_v c = 0 else True);
       assert(if uint_v cin < uint_v c then as_nat h1 result == as_nat h0 x else as_nat h1 result == as_nat h0 tempBuffer);
 
-      assert(as_nat h1 result < prime256);
+      assert(as_nat h1 result < prime);
 
-      modulo_addition_lemma (as_nat h1 result) prime256 1;
-      small_modulo_lemma_1 (as_nat h1 result) prime256; 
+      modulo_addition_lemma (as_nat h1 result) prime 1;
+      small_modulo_lemma_1 (as_nat h1 result) prime; 
   pop_frame()   
 
 
 inline_for_extraction
 val reduction_prime256_2prime256_8_with_carry_impl: x: widefelem -> result: felem -> 
   Stack unit 
-    (requires fun h -> live h x /\ live h result /\ eq_or_disjoint x result /\ wide_as_nat h x < 2 * prime256)
-    (ensures fun h0 _ h1 -> modifies (loc result) h0 h1 /\ as_nat h1 result = wide_as_nat h0 x % prime256)
+    (requires fun h -> live h x /\ live h result /\ eq_or_disjoint x result /\ wide_as_nat h x < 2 * prime)
+    (ensures fun h0 _ h1 -> modifies (loc result) h0 h1 /\ as_nat h1 result = wide_as_nat h0 x % prime)
 
 let reduction_prime256_2prime256_8_with_carry_impl x result = 
   push_frame();
     assert_norm (pow2 64 * pow2 64 * pow2 64 * pow2 64 = pow2 256);
-    assert_norm (prime256 < pow2 256);
-    assert_norm(pow2 256 < 2 * prime256);
+    assert_norm(pow2 256 < 2 * prime);
     let h0 = ST.get() in 
     let tempBuffer = create (size 4) (u64 0) in 
     let tempBufferForSubborrow = create (size 1) (u64 0) in 
@@ -88,41 +87,40 @@ let reduction_prime256_2prime256_8_with_carry_impl x result =
     let carry = sub_borrow_u64 c cin (u64 0) tempBufferForSubborrow in 
     cmovznz4 carry tempBuffer x_ result; 
       let h4 = ST.get() in 
-      assert_norm (pow2 256 > prime256);
-      assert(if (wide_as_nat h0 x < prime256) then begin
-      small_modulo_lemma_1 (wide_as_nat h0 x) prime256;
-      as_nat h4 result = (wide_as_nat h0 x) % prime256 end 
+      assert(if (wide_as_nat h0 x < prime) then begin
+      small_modulo_lemma_1 (wide_as_nat h0 x) prime;
+      as_nat h4 result = (wide_as_nat h0 x) % prime end 
       else 
 	begin 
-	small_modulo_lemma_1 (as_nat h4 result) prime256;
-	lemma_mod_sub (wide_as_nat h0 x) prime256 1;
-	as_nat h4 result = (wide_as_nat h0 x) % prime256
+	small_modulo_lemma_1 (as_nat h4 result) prime;
+	lemma_mod_sub (wide_as_nat h0 x) prime 1;
+	as_nat h4 result = (wide_as_nat h0 x) % prime
 	end );
  pop_frame()
 
-val lemma_reduction1_0: a: nat {a < pow2 256 /\ a >= prime256} -> r: nat{r = a - prime256} -> 
-  Lemma (r = a % prime256)
+val lemma_reduction1_0: a: nat {a < pow2 256 /\ a >= prime} -> r: nat{r = a - prime} -> 
+  Lemma (r = a % prime)
 
 let lemma_reduction1_0 a r = 
-  assert_norm (pow2 256 - prime256 < prime256);
-  small_modulo_lemma_1 r prime256; 
-  lemma_mod_sub_distr a prime256 prime256
+  assert_norm (pow2 256 - prime < prime);
+  small_modulo_lemma_1 r prime; 
+  lemma_mod_sub_distr a prime prime
 
 
-val lemma_reduction1: a: nat {a < pow2 256} -> r: nat{if a >= prime256 then r = a - prime256 else r = a} ->
-  Lemma (r = a % prime256)
+val lemma_reduction1: a: nat {a < pow2 256} -> r: nat{if a >= prime then r = a - prime else r = a} ->
+  Lemma (r = a % prime)
 
 let lemma_reduction1 a r = 
-  if a >= prime256 then
+  if a >= prime then
    lemma_reduction1_0 a r
   else
-    small_mod r prime256
+    small_mod r prime
 
 
 val reduction_prime_2prime_impl: x: felem -> result: felem -> 
   Stack unit
     (requires fun h -> live h x /\ live h result /\ eq_or_disjoint x result)
-    (ensures fun h0 _ h1 -> modifies (loc result) h0 h1 /\ as_nat h1 result == as_nat h0 x % prime256)
+    (ensures fun h0 _ h1 -> modifies (loc result) h0 h1 /\ as_nat h1 result == as_nat h0 x % prime)
 
 let reduction_prime_2prime_impl x result = 
   assert_norm (pow2 64 * pow2 64 * pow2 64 * pow2 64 = pow2 256);
@@ -145,7 +143,7 @@ val lemma_t_computation: t: uint64{uint_v t == 0 \/ uint_v t == 1} ->
 	let t2 = (u64 0) -. t in 
 	let t3 = (t <<. (size 32)) -. (t <<. (size 1)) in 
 	let s = uint_v t0 + uint_v t1 * pow2 64 + uint_v t2 * pow2 128 + uint_v t3 * pow2 192 in 
-	if uint_v t = 1 then s == pow2 256 - prime256 - 1 else s == 0
+	if uint_v t = 1 then s == pow2 256 - prime - 1 else s == 0
     )
 
 let lemma_t_computation t = 
@@ -154,7 +152,7 @@ let lemma_t_computation t =
   let t2 = (u64 0) -. t in 
   let t3 = (t <<. (size 32)) -. (t <<. (size 1)) in 
   let s = uint_v t0 + uint_v t1 * pow2 64 + uint_v t2 * pow2 128 + uint_v t3 * pow2 192 in  
-  assert_norm(18446744069414584320 * pow2 64 + 18446744073709551615 * pow2 128 + 4294967294 * pow2 192 = pow2 256 - prime256 - 1)
+  assert_norm(18446744069414584320 * pow2 64 + 18446744073709551615 * pow2 128 + 4294967294 * pow2 192 = pow2 256 - prime - 1)
 
 
 val lemma_t_computation2: t: uint64 {uint_v t == 0 \/ uint_v t == 1} ->
@@ -165,7 +163,7 @@ val lemma_t_computation2: t: uint64 {uint_v t == 0 \/ uint_v t == 1} ->
       let t2 = u64 0 in 
       let t3 = t -. (t <<. (size 32)) in 
       let s = uint_v t0 + uint_v t1 * pow2 64 + uint_v t2 * pow2 128 + uint_v t3 * pow2 192 in 
-      if uint_v t = 1 then s == prime256 else s == 0
+      if uint_v t = 1 then s == prime else s == 0
     )
 
 let lemma_t_computation2 t = 
@@ -174,19 +172,19 @@ let lemma_t_computation2 t =
   let t2 = u64 0 in 
   let t3 = t -. (t <<. (size 32)) in 
   let s = uint_v t0 + uint_v t1 * pow2 64 + uint_v t2 * pow2 128 + uint_v t3 * pow2 192 in  
-  assert_norm(18446744073709551615 + 4294967295 * pow2 64 + 18446744069414584321 * pow2 192 = prime256)
+  assert_norm(18446744073709551615 + 4294967295 * pow2 64 + 18446744069414584321 * pow2 192 = prime)
 
 
 val p256_add: arg1: felem -> arg2: felem ->  out: felem -> Stack unit 
   (requires (fun h0 ->  
     live h0 arg1 /\ live h0 arg2 /\ live h0 out /\ 
     eq_or_disjoint arg1 out /\ eq_or_disjoint arg2 out /\
-    as_nat h0 arg1 < prime256 /\ as_nat h0 arg2 < prime256 
+    as_nat h0 arg1 < prime /\ as_nat h0 arg2 < prime
    )
   )
   (ensures (fun h0 _ h1 -> modifies (loc out) h0 h1 /\ 
-      as_nat h1 out == (as_nat h0 arg1 + as_nat h0 arg2) % prime256 /\
-      as_nat h1 out == toDomain_ ((fromDomain_ (as_nat h0 arg1) + fromDomain_ (as_nat h0 arg2)) % prime256)
+    as_nat h1 out == (as_nat h0 arg1 + as_nat h0 arg2) % prime /\
+    as_nat h1 out == toDomain_ ((fromDomain_ (as_nat h0 arg1) + fromDomain_ (as_nat h0 arg2)) % prime)
     )
   )
 
@@ -203,10 +201,10 @@ let p256_add arg1 arg2 out =
 
 
 val p256_double: arg1: felem ->  out: felem -> Stack unit 
-  (requires (fun h0 ->  live h0 arg1 /\ live h0 out /\ eq_or_disjoint arg1 out /\ as_nat h0 arg1 < prime256))
+  (requires (fun h0 ->  live h0 arg1 /\ live h0 out /\ eq_or_disjoint arg1 out /\ as_nat h0 arg1 < prime))
   (ensures (fun h0 _ h1 -> modifies (loc out) h0 h1 /\ 
-    as_nat h1 out == (2 * as_nat h0 arg1) % prime256 /\ as_nat h1 out < prime256 /\
-    as_nat h1 out == toDomain_ (2 * fromDomain_ (as_nat h0 arg1) % prime256)
+    as_nat h1 out == (2 * as_nat h0 arg1) % prime/\ as_nat h1 out < prime /\
+    as_nat h1 out == toDomain_ (2 * fromDomain_ (as_nat h0 arg1) % prime)
   )
 )
 
@@ -224,10 +222,10 @@ val p256_sub: arg1: felem -> arg2: felem -> out: felem -> Stack unit
   (requires 
     (fun h0 -> live h0 out /\ live h0 arg1 /\ live h0 arg2 /\ 
       eq_or_disjoint arg1 out /\ eq_or_disjoint arg2 out /\
-      as_nat h0 arg1 < prime256 /\ as_nat h0 arg2 < prime256))
+      as_nat h0 arg1 < prime /\ as_nat h0 arg2 < prime))
     (ensures (fun h0 _ h1 -> modifies (loc out) h0 h1 /\ 
-	as_nat h1 out == (as_nat h0 arg1 - as_nat h0 arg2) % prime256 /\
-	as_nat h1 out == toDomain_ ((fromDomain_ (as_nat h0 arg1) - fromDomain_ (as_nat h0 arg2)) % prime256)
+      as_nat h1 out == (as_nat h0 arg1 - as_nat h0 arg2) % prime /\
+      as_nat h1 out == toDomain_ ((fromDomain_ (as_nat h0 arg1) - fromDomain_ (as_nat h0 arg2)) % prime)
     )
 )    
 
@@ -241,19 +239,19 @@ let p256_sub arg1 arg2 out =
   let t1 = ((u64 0) -. t) >>. (size 32) in 
   let t2 = u64 0 in 
   let t3 = t -. (t <<. (size 32)) in 
-    modulo_addition_lemma  (as_nat h0 arg1 - as_nat h0 arg2) prime256 1;
+    modulo_addition_lemma  (as_nat h0 arg1 - as_nat h0 arg2) prime 1;
   let c = add4_variables out (u64 0)  t0 t1 t2 t3 out in 
     let h2 = ST.get() in 
       assert(
       if as_nat h0 arg1 - as_nat h0 arg2 >= 0 then 
 	begin
-	  modulo_lemma (as_nat h0 arg1 - as_nat h0 arg2) prime256;
-	  as_nat h2 out == (as_nat h0 arg1 - as_nat h0 arg2) % prime256
+	  modulo_lemma (as_nat h0 arg1 - as_nat h0 arg2) prime;
+	  as_nat h2 out == (as_nat h0 arg1 - as_nat h0 arg2) % prime
 	end
       else
           begin
-	    modulo_lemma (as_nat h2 out) prime256;
-            as_nat h2 out == (as_nat h0 arg1 - as_nat h0 arg2) % prime256
+	    modulo_lemma (as_nat h2 out) prime;
+            as_nat h2 out == (as_nat h0 arg1 - as_nat h0 arg2) % prime
 	  end);
     substractionInDomain (felem_seq_as_nat (as_seq h0 arg1)) (felem_seq_as_nat (as_seq h0 arg2));
     inDomain_mod_is_not_mod (fromDomain_ (felem_seq_as_nat (as_seq h0 arg1)) - fromDomain_ (felem_seq_as_nat (as_seq h0 arg2)))
