specs/ecdsap256sha2/Hacl.Spec.P256.MontgomeryMultiplication.PointDouble.fst
@@ -13,27 +13,27 @@ open Lib.Loops
 open FStar.Mul
 open Hacl.Spec.P256
 
+open Spec.P256.Field
 
 #set-options "--z3rlimit 300" 
 
-let prime = prime256
-
-val lemma_xToSpecification: pxD: nat {pxD < prime256} -> pyD: nat {pyD < prime256} -> pzD: nat  {pzD < prime256} -> 
+val lemma_xToSpecification: pxD: nat {pxD < prime} -> pyD: nat {pyD < prime} -> pzD: nat {pzD < prime} -> 
   s: nat{fromDomain_ s = 4 * pxD * pyD * pyD % prime} -> 
   m: nat{fromDomain_ m = (((-3) * pzD * pzD * pzD * pzD + 3 * pxD * pxD)) % prime} -> 
   x3: nat{
     let mD = fromDomain_ m in 
     let sD = fromDomain_ s in 
-    fromDomain_ x3 = (mD * mD - 2*sD) % prime} -> 
-  Lemma (
-    (let (xN, yN, zN) = _point_double (pxD, pyD, pzD) in 
+    fromDomain_ x3 = (mD * mD - 2 * sD) % prime} -> 
+  Lemma 
+    (
+      (let (xN, yN, zN) = _point_double (pxD, pyD, pzD) in 
       fromDomain_ x3 = xN)
     )
 
 let lemma_xToSpecification pxD pyD pzD s m x3 = ()
 
 
-val lemma_yToSpecification: pxD: nat {pxD < prime256} -> pyD: nat {pyD < prime256} -> pzD: nat  {pzD < prime256} ->
+val lemma_yToSpecification: pxD: nat {pxD < prime} -> pyD: nat {pyD < prime} -> pzD: nat {pzD < prime} ->
   s: nat {s = toDomain_ (4 * pxD * pyD * pyD % prime)} -> 
   m: nat {m = toDomain_ (((-3) * pzD * pzD * pzD * pzD + 3 * pxD * pxD) % prime)} ->
   x3: nat{
@@ -52,9 +52,10 @@ val lemma_yToSpecification: pxD: nat {pxD < prime256} -> pyD: nat {pyD < prime25
 let lemma_yToSpecification pxD pyD pzD s m x3 y3 = ()
 
 
-val lemma_zToSpecification: pxD: nat {pxD < prime256} -> pyD: nat {pyD < prime256} -> pzD: nat  {pzD < prime256} ->
+val lemma_zToSpecification: pxD: nat {pxD < prime} -> pyD: nat {pyD < prime} -> pzD: nat {pzD < prime} ->
   z3: nat{fromDomain_ z3 = 2 * pyD * pzD % prime} -> 
-  Lemma (
+  Lemma 
+  (
     let (xN, yN, zN) = _point_double (pxD, pyD, pzD) in 
     fromDomain_ z3 = zN
   )
