specs/ecdsap256sha2/Hacl.Spec.P256.fst
@@ -9,6 +9,8 @@ open Lib.Sequence
 open Hacl.Spec.P256.Definitions
 open Hacl.Spec.P256.Lemmas
 
+open Spec.P256.Field
+
 #set-options "--fuel 0 --ifuel 0 --z3rlimit 100"
 
 (*
@@ -18,16 +20,14 @@ y^2 = x^3-3x+4105836372515214212932612978004726840911444101599372555483525631403
 
 modulo p = 2^256 - 2^224 + 2^192 + 2^96 - 1 *)
 
-let prime = prime256
-
 let aCoordinateP256 = -3 
-let bCoordinateP256 : (a: nat {a < prime256}) =
-  assert_norm (41058363725152142129326129780047268409114441015993725554835256314039467401291 < prime256);
+let bCoordinateP256 : (a: nat {a < prime}) =
+  assert_norm (41058363725152142129326129780047268409114441015993725554835256314039467401291 < prime);
   41058363725152142129326129780047268409114441015993725554835256314039467401291
 
 noextract
 let basePoint : point_nat_prime =
-  assert_norm (0x6B17D1F2E12C4247F8BCE6E563A440F277037D812DEB33A0F4A13945D898C296 < prime256);
+  assert_norm (0x6B17D1F2E12C4247F8BCE6E563A440F277037D812DEB33A0F4A13945D898C296 < prime);
   (0x6B17D1F2E12C4247F8BCE6E563A440F277037D812DEB33A0F4A13945D898C296,
    0x4FE342E2FE1A7F9B8EE7EB4A7C0F9E162BCE33576B315ECECBB6406837BF51F5,
    1)
@@ -36,11 +36,11 @@ let basePoint : point_nat_prime =
 noextract
 let _point_double (p:point_nat_prime) : point_nat_prime =
   let x, y, z = p in
-  let s = (4 * x * y * y) % prime256 in
-  let m = ((-3) * z * z * z * z + 3 * x * x) % prime256 in
-  let x3 = (m * m - 2 * s) % prime256 in
-  let y3 = (m * (s - x3) - 8 * y * y * y * y) % prime256 in
-  let z3 = (2 * y * z) % prime256 in
+  let s = (4 * x * y * y) % prime in
+  let m = ((-3) * z * z * z * z + 3 * x * x) % prime in
+  let x3 = (m * m - 2 * s) % prime in
+  let y3 = (m * (s - x3) - 8 * y * y * y * y) % prime in
+  let z3 = (2 * y * z) % prime in
   (x3, y3, z3)
 
 
@@ -55,20 +55,20 @@ let _point_add (p:point_nat_prime) (q:point_nat_prime) : point_nat_prime =
   let z2z2 = z2 * z2 in
   let z1z1 = z1 * z1 in
 
-  let u1 = x1 * z2z2 % prime256 in
-  let u2 = x2 * z1z1 % prime256 in
+  let u1 = x1 * z2z2 % prime in
+  let u2 = x2 * z1z1 % prime in
 
   assert_by_tactic (x1 * z2 * z2 = x1 * (z2 * z2)) canon;
   assert_by_tactic (x2 * z1 * z1 = x2 * (z1 * z1)) canon;
 
-  let s1 = y1 * z2 * z2z2 % prime256 in
-  let s2 = y2 * z1 * z1z1 % prime256 in
+  let s1 = y1 * z2 * z2z2 % prime in
+  let s2 = y2 * z1 * z1z1 % prime in
 
   assert_by_tactic (y1 * z2 * (z2 * z2) = y1 * z2 * z2 * z2) canon;
   assert_by_tactic (y2 * z1 * (z1 * z1) = y2 * z1 * z1 * z1) canon;
 
-  let h = (u2 - u1) % prime256 in
-  let r = (s2 - s1) % prime256 in
+  let h = (u2 - u1) % prime in
+  let r = (s2 - s1) % prime in
 
   let rr = (r * r) in
   let hh = (h * h) in
@@ -76,11 +76,11 @@ let _point_add (p:point_nat_prime) (q:point_nat_prime) : point_nat_prime =
 
   assert_by_tactic (forall (n: nat). n * h * h = n * (h * h)) canon;
   assert_by_tactic (s1 * (h * h * h) = s1 * h * h * h) canon;
-  let x3 = (rr - hhh - 2 * u1 * hh) % prime256 in
-  assert(x3 = (r * r - h * h * h - 2 * u1 * h * h) % prime256);
-  let y3 = (r * (u1 * hh - x3) - s1 * hhh) % prime256 in
-  assert(y3 = (r * (u1 * h*h - x3) - s1 * h*h*h) % prime256);
-  let z3 = (h * z1 * z2) % prime256 in
+  let x3 = (rr - hhh - 2 * u1 * hh) % prime in
+  assert(x3 = (r * r - h * h * h - 2 * u1 * h * h) % prime);
+  let y3 = (r * (u1 * hh - x3) - s1 * hhh) % prime in
+  assert(y3 = (r * (u1 * h*h - x3) - s1 * h*h*h) % prime);
+  let z3 = (h * z1 * z2) % prime in
   if z2 = 0 then
     (x1, y1, z1)
   else
@@ -95,17 +95,17 @@ let isPointAtInfinity (p:point_nat) =
 
 
 let _norm (p:point_nat_prime) : point_nat_prime =
-  assert_norm (prime256 - 2 > 0);
+  assert_norm (prime - 2 > 0);
   let (x, y, z) = p in
   let z2 = z * z in
   let z2i = modp_inv2_pow z2 in
   let z3 = z * z * z in
   let z3i = modp_inv2_pow z3 in
-  let x3 = (z2i * x) % prime256 in
-  let y3 = (z3i * y) % prime256 in
+  let x3 = (z2i * x) % prime in
+  let y3 = (z3i * y) % prime in
   let z3 = if isPointAtInfinity p then 0 else 1 in
-  assert(x3 == (x * (pow (z * z) (prime256 - 2) % prime256) % prime256));
-  assert(y3 == (y * (pow (z * z * z) (prime256 - 2) % prime256) % prime256));
+  (*assert(x3 == (x * (pow (z * z) (prime - 2) % prime) % prime));
+  assert(y3 == (y * (pow (z * z * z) (prime - 2) % prime) % prime)); *)
   (x3, y3, z3)
 
 
