code/ecdsap256sha2/Hacl.Impl.P256.Arithmetics.fsti
@@ -19,25 +19,27 @@ open Hacl.Spec.P256.MontgomeryMultiplication
 
 open FStar.Math.Lemmas
 
+open Spec.P256.Field
+
 open FStar.Mul
 
 val quatre: a: felem -> result: felem -> Stack unit
   (requires fun h -> live h a /\ live h result /\ disjoint a result /\ as_nat h a < prime)
   (ensures fun h0 _ h1 -> modifies (loc result) h0 h1 /\ 
-    as_nat h1 result = toDomain_ (fromDomain_ (as_nat h0 a) * fromDomain_ (as_nat h0 a) * fromDomain_ (as_nat h0 a) * fromDomain_ (as_nat h0 a) % prime256) /\ 
+    as_nat h1 result = toDomain_ (fromDomain_ (as_nat h0 a) * fromDomain_ (as_nat h0 a) * fromDomain_ (as_nat h0 a) * fromDomain_ (as_nat h0 a) % prime) /\ 
     as_nat h1 result = toDomain_ (fromDomain_ (as_nat h0 a) * fromDomain_ (as_nat h0 a) * fromDomain_ (as_nat h0 a) * fromDomain_ (as_nat h0 a)))
 
 val multByTwo: a: felem -> result: felem -> Stack unit 
   (requires fun h -> live h a /\ live h result /\ eq_or_disjoint a result /\ as_nat h a < prime )
   (ensures fun h0 _ h1 -> modifies (loc result) h0 h1 /\ 
-    as_nat h1 result == toDomain_ (2 * fromDomain_ (as_nat h0 a) % prime256) /\ 
+    as_nat h1 result == toDomain_ (2 * fromDomain_ (as_nat h0 a) % prime) /\ 
     as_nat h1 result == toDomain_ (2 * fromDomain_ (as_nat h0 a)) /\ 
     as_nat h1 result < prime)
 
 val multByThree: a: felem -> result: felem -> Stack unit 
   (requires fun h -> live h a /\ live h result /\ disjoint a result /\ as_nat h a < prime )
   (ensures fun h0 _ h1 -> modifies (loc result) h0 h1 /\ as_nat h1 result < prime /\ 
-    as_nat h1 result == toDomain_ (3 * fromDomain_ (as_nat h0 a) % prime256) /\ 
+    as_nat h1 result == toDomain_ (3 * fromDomain_ (as_nat h0 a) % prime) /\ 
     as_nat h1 result == toDomain_ (3 * fromDomain_ (as_nat h0 a))
   )
 
@@ -45,14 +47,14 @@ val multByThree: a: felem -> result: felem -> Stack unit
 val multByFour: a: felem -> result: felem -> Stack unit 
   (requires fun h -> live h a /\ live h result /\ eq_or_disjoint a result /\ as_nat h a < prime )
   (ensures fun h0 _ h1 -> modifies (loc result) h0 h1 /\ as_nat h1 result < prime /\ 
-    as_nat h1 result == toDomain_ (4 * fromDomain_ (as_nat h0 a) % prime256) /\ 
+    as_nat h1 result == toDomain_ (4 * fromDomain_ (as_nat h0 a) % prime) /\ 
     as_nat h1 result == toDomain_ (4 * fromDomain_ (as_nat h0 a))
 )
 
 val multByEight: a: felem -> result: felem -> Stack unit 
   (requires fun h -> live h a /\ live h result /\ disjoint a result /\ as_nat h a < prime )
   (ensures fun h0 _ h1 -> modifies (loc result) h0 h1 /\ as_nat h1 result < prime /\ 
-    as_nat h1 result == toDomain_ (8 * fromDomain_ (as_nat h0 a) % prime256) /\ 
+    as_nat h1 result == toDomain_ (8 * fromDomain_ (as_nat h0 a) % prime) /\ 
     as_nat h1 result == toDomain_ (8 * fromDomain_ (as_nat h0 a))
 )
 
@@ -60,5 +62,5 @@ val multByMinusThree: a: felem -> result: felem -> Stack unit
   (requires fun h -> live h a /\ live h result /\ disjoint a result /\ as_nat h a < prime )
   (ensures fun h0 _ h1 -> modifies (loc result) h0 h1 /\ 
     as_nat h1 result < prime /\ 
-    as_nat h1 result == toDomain_ ((-3) * fromDomain_ (as_nat h0 a) % prime256) /\
+    as_nat h1 result == toDomain_ ((-3) * fromDomain_ (as_nat h0 a) % prime) /\
     as_nat h1 result == toDomain_ ((-3) * fromDomain_ (as_nat h0 a)))
