code/ecdsap256sha2/Hacl.Impl.P256.DH.fst
@@ -18,6 +18,8 @@ open Hacl.Impl.LowLevel
 open Hacl.Impl.P256
 open Hacl.Impl.P256.Signature.Common
 
+open Spec.P256.Field
+
 #set-options "--fuel 0 --ifuel 0 --z3rlimit 100"
 
 let ecp256dh_i result scalar =
@@ -71,7 +73,7 @@ val _ecp256dh_r:
        if not (verifyQValidCurvePointSpec (pointJacX, pointJacY, pointJacZ)) then
          uint_v r = maxint U64 /\ x3 == 0 /\ y3 == 0
        else
-        x3 < prime256 /\ y3 < prime256 /\ z3 < prime256 /\
+        x3 < prime /\ y3 < prime /\ z3 < prime /\
         (let xN, yN, zN = scalar_multiplication (as_seq h0 scalar) (pointJacX, pointJacY, pointJacZ) in
          xN == x3 /\ yN == y3 /\ zN == z3 /\
          (if isPointAtInfinity (xN, yN, zN) then
