code/ecdsap256sha2/Hacl.Impl.P256.PointAdd.fst
@@ -21,7 +21,7 @@ open Hacl.Impl.P256.MontgomeryMultiplication
 open Hacl.Spec.P256
 open Hacl.Impl.P256.Math 
 
-
+open Spec.P256.Field
 open FStar.Tactics 
 open FStar.Tactics.Canon
 
