code/ecdsap256sha2/Hacl.Impl.P256.fsti
@@ -24,6 +24,8 @@ open Hacl.Spec.P256
 open Lib.Loops
 open FStar.Math.Lemmas
 
+open Spec.P256.Field
+
 module B = LowStar.Buffer
 open FStar.Mul
 
@@ -152,9 +154,9 @@ val scalarMultiplication: #buf_type: buftype->  p: point -> result: point ->
   (ensures fun h0 _ h1 -> 
     modifies3 p result tempBuffer h0 h1 /\ 
     modifies (loc p |+| loc result |+| loc tempBuffer) h0 h1 /\
-    as_nat h1 (gsub result (size 0) (size 4)) < prime256 /\ 
-    as_nat h1 (gsub result (size 4) (size 4)) < prime256 /\
-    as_nat h1 (gsub result (size 8) (size 4)) < prime256 /\
+    as_nat h1 (gsub result (size 0) (size 4)) < prime /\ 
+    as_nat h1 (gsub result (size 4) (size 4)) < prime /\
+    as_nat h1 (gsub result (size 8) (size 4)) < prime /\
     (
       let x3, y3, z3 = point_x_as_nat h1 result, point_y_as_nat h1 result, point_z_as_nat h1 result in 
       let (xN, yN, zN) = scalar_multiplication (as_seq h0 scalar) (point_prime_to_coordinates (as_seq h0 p)) in 
@@ -177,9 +179,9 @@ val scalarMultiplicationWithoutNorm: p: point -> result: point ->
   (ensures fun h0 _ h1 -> 
     modifies (loc p |+| loc result |+| loc tempBuffer) h0 h1 /\ 
     
-    as_nat h1 (gsub result (size 0) (size 4)) < prime256 /\ 
-    as_nat h1 (gsub result (size 4) (size 4)) < prime256 /\
-    as_nat h1 (gsub result (size 8) (size 4)) < prime256 /\
+    as_nat h1 (gsub result (size 0) (size 4)) < prime /\ 
+    as_nat h1 (gsub result (size 4) (size 4)) < prime /\
+    as_nat h1 (gsub result (size 8) (size 4)) < prime /\
     
     modifies (loc p |+| loc result |+| loc tempBuffer) h0 h1 /\
     (
