code/ecdsap256sha2/Hacl.Impl.SolinasReduction.fst
@@ -19,6 +19,8 @@ open FStar.Mul
 module BV = FStar.BitVector
 module Seq = FStar.Seq
 
+open Spec.P256.Field
+
 #reset-options "--fuel 0 --ifuel 0 --z3rlimit 50"
 
 inline_for_extraction noextract
@@ -132,8 +134,8 @@ val upl_zer_buffer:
       live h o /\ live h temp /\ disjoint o temp)
     (ensures fun h0 _ h1 ->
       modifies (loc o |+| loc temp) h0 h1 /\
-      as_nat h1 o == (v c0 + v c1 * pow2 (1 * 32) + v c2 * pow2 (2 * 32) + v c3 * pow2 (3 * 32) + v c4 * pow2 (4 * 32) + v c5 * pow2 (5 * 32) + v  c6 * pow2 (6 * 32) + v c7 * pow2 (7 * 32)) % prime256
-   )
+      as_nat h1 o == (v c0 + v c1 * pow2 (1 * 32) + v c2 * pow2 (2 * 32) + v c3 * pow2 (3 * 32) + v c4 * pow2 (4 * 32) + v c5 * pow2 (5 * 32) + v  c6 * pow2 (6 * 32) + v c7 * pow2 (7 * 32)) % prime
+    )
 
 let upl_zer_buffer c0 c1 c2 c3 c4 c5 c6 c7 temp o =
     let b0 = store_high_low_u c1 c0 in
@@ -154,7 +156,7 @@ let upl_zer_buffer c0 c1 c2 c3 c4 c5 c6 c7 temp o =
     load_buffer b0 b1 b2 b3 temp;
     reduction_prime_2prime_impl temp o;
     let h2 = ST.get() in
-    assert(as_nat h2 o = (v c1 * pow2 32 + v c0 + v c3 * pow2 (3 * 32) + v c2 * pow2 (2 * 32) + v c5 * pow2 (32 * 5) + v c4 * pow2 (32 * 4) + v c7 * pow2 (32 * 7) + v c6 * pow2 (32 * 6)) % prime256)
+    assert(as_nat h2 o = (v c1 * pow2 32 + v c0 + v c3 * pow2 (3 * 32) + v c2 * pow2 (2 * 32) + v c5 * pow2 (32 * 5) + v c4 * pow2 (32 * 4) + v c7 * pow2 (32 * 7) + v c6 * pow2 (32 * 6)) % prime)
 
 
 val upl_fir_buffer: c11: uint32 -> c12: uint32 -> c13: uint32 -> c14: uint32 -> c15: uint32
@@ -164,7 +166,7 @@ val upl_fir_buffer: c11: uint32 -> c12: uint32 -> c13: uint32 -> c14: uint32 -> 
     (requires fun h -> live h o /\ live h temp /\ disjoint o temp)
     (ensures fun h0 _ h1 ->
       modifies (loc o |+| loc temp) h0 h1 /\
-      as_nat h1 o == (v c11 * pow2 (3 * 32) + v c12 * pow2 (4 * 32) + v c13 * pow2 (5 * 32) + v c14 * pow2 (6 * 32) + v c15 * pow2 (7 * 32)) % prime256
+      as_nat h1 o == (v c11 * pow2 (3 * 32) + v c12 * pow2 (4 * 32) + v c13 * pow2 (5 * 32) + v c14 * pow2 (6 * 32) + v c15 * pow2 (7 * 32)) % prime
     )
 
 let upl_fir_buffer c11 c12 c13 c14 c15 temp o =
@@ -213,7 +215,7 @@ val upl_thi_buffer: c8: uint32 -> c9: uint32 -> c10: uint32 -> c14: uint32 -> c1
   Stack unit
  (requires fun h -> live h o /\ live h temp /\ disjoint o temp)
  (ensures fun h0 _ h1 -> modifies2 o temp h0 h1 /\
-      as_nat h1 o == (v c8 + v c9 * pow2 32 + v c10 * pow2 (2 * 32) +  v c14 * pow2 (6 * 32) + v c15 * pow2 (7 * 32)) % prime256)
+      as_nat h1 o == (v c8 + v c9 * pow2 32 + v c10 * pow2 (2 * 32) +  v c14 * pow2 (6 * 32) + v c15 * pow2 (7 * 32)) % prime)
 
 let upl_thi_buffer c8 c9 c10 c14 c15 temp o =
    assert_norm (pow2 (1 * 32) * pow2 (2 * 32) = pow2 (3 * 32));
@@ -236,7 +238,7 @@ val upl_for_buffer: c8: uint32 -> c9: uint32 -> c10: uint32 -> c11: uint32 -> c1
   Stack unit
     (requires fun h -> live h o /\ live h temp /\ disjoint o temp)
     (ensures fun h0 _ h1 -> modifies2 o temp h0 h1 /\
-        as_nat h1 o == (v c9 + v c10 * pow2 32 + v c11 * pow2 (2 * 32) + v c13 * pow2 (3 * 32) + v c14 * pow2 (4 * 32) + v c15 * pow2 (5 * 32) + v c13 * pow2 (6 * 32) +  v c8 * pow2 (7 * 32)) % prime256)
+        as_nat h1 o == (v c9 + v c10 * pow2 32 + v c11 * pow2 (2 * 32) + v c13 * pow2 (3 * 32) + v c14 * pow2 (4 * 32) + v c15 * pow2 (5 * 32) + v c13 * pow2 (6 * 32) +  v c8 * pow2 (7 * 32)) % prime)
 
 let upl_for_buffer c8 c9 c10 c11 c13 c14 c15 temp o =
   assert_norm (pow2 (1 * 32) * pow2 (2 * 32) = pow2 (3 * 32));
@@ -258,7 +260,7 @@ val upl_fif_buffer: c8: uint32 -> c10: uint32 -> c11: uint32 -> c12: uint32 -> c
   Stack unit
     (requires fun h -> live h o /\ live h temp /\ disjoint o temp)
     (ensures fun h0 _ h1 -> modifies2 o temp h0 h1 /\
-    as_nat h1 o == (v c11 + v c12 * pow2 32 + v c13 * pow2 (2 * 32) + v c8 * pow2 (6 * 32) + v c10 * pow2 (7 * 32)) % prime256)
+    as_nat h1 o == (v c11 + v c12 * pow2 32 + v c13 * pow2 (2 * 32) + v c8 * pow2 (6 * 32) + v c10 * pow2 (7 * 32)) % prime)
 
 let upl_fif_buffer c8 c10 c11 c12 c13 temp o =
      assert_norm (pow2 (1 * 32) * pow2 (2 * 32) = pow2 (3 * 32));
@@ -281,7 +283,7 @@ val upl_six_buffer: c9: uint32 -> c11: uint32 -> c12: uint32 -> c13: uint32 -> c
     (requires fun h -> live h o /\ live h temp /\ disjoint o temp)
     (ensures fun h0 _ h1 -> modifies2 o temp h0 h1 /\ as_nat h1 o == (
     v c12 + v c13 * pow2 32 + v c14 * pow2 (2 * 32) + v c15 * pow2 (3 * 32) +
-          v c9 * pow2 (6 * 32) + v c11 * pow2 (7 * 32)) % prime256)
+          v c9 * pow2 (6 * 32) + v c11 * pow2 (7 * 32)) % prime)
 
 let upl_six_buffer c9 c11 c12 c13 c14 c15 temp o =
   assert_norm (pow2 (1 * 32) * pow2 (2 * 32) = pow2 (3 * 32));
@@ -304,7 +306,7 @@ val upl_sev_buffer: c8: uint32 -> c9: uint32 -> c10: uint32 -> c12: uint32 -> c1
   Stack unit
     (requires fun h -> live h o /\ live h temp /\ disjoint o temp)
       (ensures fun h0 _ h1 -> modifies2 o temp h0 h1 /\
-        as_nat h1 o == (v c13 + v c14 * pow2 32 + v c15 * pow2 (2 * 32) + v c8 * pow2 (3 * 32) +  v c9 * pow2 (4 * 32) + v c10 * pow2 (5 * 32) + v c12 * pow2 (7 * 32)) % prime256)
+        as_nat h1 o == (v c13 + v c14 * pow2 32 + v c15 * pow2 (2 * 32) + v c8 * pow2 (3 * 32) +  v c9 * pow2 (4 * 32) + v c10 * pow2 (5 * 32) + v c12 * pow2 (7 * 32)) % prime)
 
 let upl_sev_buffer c8 c9 c10 c12 c13 c14 c15 temp o =
   assert_norm (pow2 (1 * 32) * pow2 (2 * 32) = pow2 (3 * 32));
@@ -326,7 +328,7 @@ val upl_eig_buffer: c9: uint32 -> c10: uint32 -> c11: uint32 -> c12: uint32 -> c
   -> o: lbuffer uint64 (size 4) ->
   Stack unit
     (requires fun h -> live h o /\ live h temp /\ disjoint o temp)
-    (ensures fun h0 _ h1 -> modifies2 o temp h0 h1 /\ as_nat h1 o == (v c14 + v c15 * pow2 32 + v c9 * pow2 (3 * 32) + v c10 * pow2 (4 * 32) + v c11 * pow2 (5 * 32) + v c13 * pow2 (7 * 32)) % prime256)
+    (ensures fun h0 _ h1 -> modifies2 o temp h0 h1 /\ as_nat h1 o == (v c14 + v c15 * pow2 32 + v c9 * pow2 (3 * 32) + v c10 * pow2 (4 * 32) + v c11 * pow2 (5 * 32) + v c13 * pow2 (7 * 32)) % prime)
 
 let upl_eig_buffer c9 c10 c11 c12 c13 c14 c15 temp o =
   assert_norm (pow2 (1 * 32) * pow2 (2 * 32) = pow2 (3 * 32));
