specs/ecdsap256sha2/Hacl.Spec.P256.MontgomeryMultiplication.fsti
@@ -9,9 +9,10 @@ open Hacl.Spec.P256.Definitions
 
 open Lib.IntTypes
 
+open Spec.P256.Field
 
 noextract
-val fromDomain_: a: int -> Tot (a: nat {a < prime256})
+val fromDomain_: a: int -> Tot (a: nat {a < prime})
 
 noextract
 val fromDomainPoint: a: tuple3 nat nat nat -> Tot (r: tuple3 nat nat nat 
@@ -25,29 +26,29 @@ val fromDomainPoint: a: tuple3 nat nat nat -> Tot (r: tuple3 nat nat nat
 noextract
 val toDomain_: a: int -> Tot nat
 
-val lemmaFromDomain: a: int -> Lemma (fromDomain_ (a) == a * modp_inv2 (pow2 256) % prime256)
+val lemmaFromDomain: a: int -> Lemma (fromDomain_ (a) == a * modp_inv2 (pow2 256) % prime)
 
-val lemmaToDomain: a: int -> Lemma (toDomain_(a) == a * (pow2 256) % prime256)
+val lemmaToDomain: a: int -> Lemma (toDomain_(a) == a * (pow2 256) % prime)
 
-val lemmaToDomainAndBackIsTheSame: a: nat {a < prime256} -> Lemma (fromDomain_ (toDomain_ a) == a)
+val lemmaToDomainAndBackIsTheSame: a: nat {a < prime} -> Lemma (fromDomain_ (toDomain_ a) == a)
   [SMTPat (fromDomain_ (toDomain_ a))]
 
-val lemmaFromDomainToDomain: a: nat { a < prime256} -> Lemma (toDomain_ (fromDomain_ a) == a)
+val lemmaFromDomainToDomain: a: nat { a < prime} -> Lemma (toDomain_ (fromDomain_ a) == a)
 
-val lemmaFromDomainToDomainModuloPrime: a: int -> Lemma (a % prime256 == fromDomain_(toDomain_ a))
+val lemmaFromDomainToDomainModuloPrime: a: int -> Lemma (a % prime == fromDomain_(toDomain_ a))
 
-val inDomain_mod_is_not_mod: a: int -> Lemma (toDomain_ a == toDomain_ (a % prime256))
+val inDomain_mod_is_not_mod: a: int -> Lemma (toDomain_ a == toDomain_ (a % prime))
 
 val multiplicationInDomainNat: #k: nat -> #l: nat ->
-  a: nat {a == toDomain_ k /\ a < prime256} -> 
-  b: nat {b == toDomain_ l /\ b < prime256} ->
+  a: nat {a == toDomain_ k /\ a < prime} -> 
+  b: nat {b == toDomain_ l /\ b < prime} ->
   Lemma (
-    let multResult = a * b * modp_inv2_prime (pow2 256) prime256 % prime256 in 
+    let multResult = a * b * modp_inv2_prime (pow2 256) prime % prime in 
     multResult == toDomain_ (k * l))
 
-val additionInDomain: a: nat {a < prime256} -> b: nat {b < prime256} -> Lemma 
-  ((a + b) % prime256 == toDomain_ (fromDomain_ a + fromDomain_ b))
+val additionInDomain: a: nat {a < prime} -> b: nat {b < prime} -> Lemma 
+  ((a + b) % prime == toDomain_ (fromDomain_ a + fromDomain_ b))
   
-val substractionInDomain: a: nat {a < prime256} -> b: nat { b < prime256} -> Lemma 
-  ((a - b) % prime256 == toDomain_ (fromDomain_ a - fromDomain_ b))
+val substractionInDomain: a: nat {a < prime} -> b: nat { b < prime} -> Lemma 
+  ((a - b) % prime == toDomain_ (fromDomain_ a - fromDomain_ b))
 
